

# Chapter 1

## ThermoS26-05

### 1.1 Examples

**Example 1.1.1.** (3.4) Suppose that the fundamental relation for a material is given by

$$\tilde{S} = 4A U^{1/4} V^{1/2} N^{1/4} + B N, \quad \Sigma_U = [0, \infty)^3,$$

where  $A, B > 0$  are constants. This function must be homogenous of degree one. Suppose  $\lambda > 0$ . Then

$$\tilde{S}(\lambda U, \lambda V, \lambda N) = 4A \lambda U^{1/4} \lambda V^{1/2} \lambda N^{1/4} + B \lambda N = \lambda \tilde{S}(U, V, N).///$$

Recall that

$$T = \frac{1}{\frac{\partial \tilde{S}}{\partial U}} = \left( A U^{-3/4} V^{1/2} N^{1/4} \right)^{-1} = \frac{U^{3/4}}{A V^{1/2} N^{1/4}},$$

which is homogenous degree zero.

$$\frac{P}{T} = \frac{\partial \tilde{S}}{\partial V}$$

so

$$P = T \frac{\partial \tilde{S}}{\partial V} = \frac{U^{3/4}}{A V^{1/2} N^{1/4}} \left( \frac{2A U^{1/4} N^{1/4}}{V^{1/2}} \right) = \frac{2U}{V}.$$

Finally,

$$\mu = -T \frac{\partial \tilde{S}}{\partial N} = -\frac{U^{3/4}}{A V^{1/2} N^{1/4}} \left( \frac{A U^{1/4} V^{1/2}}{N^{3/4}} + B \right) = -\frac{U}{N} - \frac{B U^{3/4}}{A V^{1/2} N^{1/4}}.///$$

**Example 1.1.2.** (3.5) Suppose that the fundamental relation is

$$\tilde{U} = \left( \frac{S - BN}{4AV^{1/2}N^{1/4}} \right)^4.$$

Recall that

$$T = \frac{\partial \tilde{U}}{\partial S} = 4 \left( \frac{S - BN}{4AV^{1/2}N^{1/4}} \right)^3 \frac{1}{4AV^{1/2}N^{1/4}} = \frac{\tilde{U}^{3/4}}{AV^{1/2}N^{1/4}},$$

the same as above.

$$P = -\frac{\partial \tilde{U}}{\partial V} = -4 \left( \frac{S - BN}{4AV^{1/2}N^{1/4}} \right)^3 \left( \frac{S - BN}{4AN^{1/4}} \right) \left( -\frac{1}{2} \right) \frac{1}{V^{3/2}}$$

so

$$= 2 \left( \frac{S - BN}{4AV^{1/2}N^{1/4}} \right)^4 \frac{1}{V} = \frac{2\tilde{U}}{V}.$$

Finally,

$$\begin{aligned} \mu = \frac{\partial \tilde{U}}{\partial N} &= 4 \left( \frac{S - BN}{4AV^{1/2}N^{1/4}} \right)^3 \frac{1}{4AV^{1/2}} \frac{N^{1/4}(-B) - (S - BN)\frac{1}{4}N^{-3/4}}{N^{1/2}} \\ &= 4 \left( \frac{S - BN}{4AV^{1/2}N^{1/4}} \right)^3 \frac{1}{4AV^{1/2}} \frac{N^{1/4}(-B) - (S - BN)\frac{1}{4}N^{-3/4}}{N^{1/2}} \\ &= 4\tilde{U}^{3/4} \frac{N^{1/4}}{4AV^{1/2}N^{1/2}} \cdot \left( -B - \frac{S - BN}{4N} \right) \\ &= -\frac{B\tilde{U}^{3/4}}{AV^{1/2}N^{1/4}} - \frac{\tilde{U}^{3/4}}{AV^{1/2}N^{1/4}} \frac{(S - BN)}{4N} = -\frac{B\tilde{U}^{3/4}}{AV^{1/2}N^{1/4}} - \frac{\tilde{U}}{N}. \end{aligned}$$

## 1.2 Euler Equation with Respect to Entropy

**Theorem 1.2.1.** (3.5) Let  $\tilde{S}$  be the internal energy of an isolated system. Then

$$\tilde{S} = \frac{1}{T_S} U + \frac{P_S}{T_S} V - \sum_{i=1}^r \frac{\mu_{S,i}}{T_S} N_i, \quad (3.8)$$

where

$$T_S = T_S(U, V, \vec{N}), \quad P_S = P_S(U, V, \vec{N}), \quad \mu_{S,i} = \mu_{S,i}(U, V, \vec{N}),$$

and

$$\frac{1}{T_S} = \frac{\partial \tilde{S}}{\partial U}, \quad \frac{P_S}{T_S} = \frac{\partial \tilde{S}}{\partial V}, \quad \frac{\mu_{S,i}}{T_S} = \frac{\partial \tilde{S}}{\partial N_i}.$$

*Proof.* We again use the fact that  $\tilde{S}$  is homogenous of degree one. For any  $\lambda > 0$ ,

$$\tilde{S}(\lambda U, \lambda V, \lambda \vec{N}) = \lambda \tilde{S}(U, V, \vec{N}).$$

Taking the derivative with respect to  $\lambda$ , we have

$$\frac{U}{T_S(\lambda U, \lambda V, \lambda \vec{N})} + \frac{P_S(\lambda U, \lambda V, \lambda \vec{N})}{T_S(\lambda U, \lambda V, \lambda \vec{N})} V + \sum_{j=1}^r \frac{\mu_{S,j}(\lambda U, \lambda V, \lambda \vec{N})}{T_S(\lambda U, \lambda V, \lambda \vec{N})} N_j = \tilde{S}(U, V, \vec{N}),$$

and setting  $\lambda = 1$  gives the desired result. ///

□

### 1.3 Gibbs-Duhem Relation in the Entropy Form

The Gibbs-Duhem equation is similarly derived.

**Theorem 1.3.1.** (3.6) Suppose that  $\vec{Y} : [0, 1] \rightarrow \Sigma_U$  is a process path. Then

$$0 = \frac{dT_S}{d\gamma}(\vec{Y}(\gamma)) \tilde{S}(\vec{Y}(\gamma)) - \frac{dP_S}{d\gamma}(\vec{Y}(\gamma)) V(\gamma) + \sum_{j=1}^r \frac{d\mu_{S,j}}{d\gamma}(\vec{Y}(\gamma)) N_j(\gamma). \quad (3.9)$$

This equation is called the Gibbs-Duhem relation in the entropy form.

*Proof.* Using (3.8), we have

$$T_S(\vec{Y}(\gamma)) \tilde{S}(\vec{Y}(\gamma)) = U(\gamma) + P_S(\vec{Y}(\gamma)) V(\gamma) - \sum_{j=1}^r \mu_{S,j}(\vec{Y}(\gamma)) N_j(\gamma).$$

Taking the  $\gamma$ -derivative of the last equation, we have

$$\begin{aligned} \frac{dT_S}{d\gamma}(\vec{Y}(\gamma)) \tilde{S}(\vec{Y}(\gamma)) + T_S(\vec{Y}(\gamma)) \frac{d\tilde{S}}{d\gamma}(\vec{Y}(\gamma)) &= U'(\gamma) + \frac{dP_S}{d\gamma}(\vec{Y}(\gamma)) V(\gamma) + P_S(\vec{Y}(\gamma)) V'(\gamma) \\ &\quad - \sum_{j=1}^r \left\{ \frac{d\mu_{S,j}}{d\gamma}(\vec{Y}(\gamma)) N_j(\gamma) + \mu_{S,j}(\vec{Y}(\gamma)) N_j'(\gamma) \right\}. \end{aligned} \quad (3.10)$$

Taking the  $\gamma$ -derivative of  $\tilde{S}(\vec{Y}(\gamma))$  we have

$$\frac{d\tilde{S}}{d\gamma}(\vec{Y}(\gamma)) = \frac{1}{T_S(\vec{Y}(\gamma))} U'(\gamma) + \frac{P_S(\vec{Y}(\gamma))}{T_S(\vec{Y}(\gamma))} V'(\gamma) - \sum_{j=1}^r \frac{\mu_{S,j}(\vec{Y}(\gamma))}{T_S(\vec{Y}(\gamma))} N_j'(\gamma). \quad (3.11)$$

Substituting (3.11) into (3.10) yields (3.9). ///

□

Remark: Compare (??) and (3.9):

$$0 = S(\gamma) \frac{dT_S(\vec{Y}(\gamma))}{d\gamma} - V(\gamma) \frac{dP_S(\vec{Y}(\gamma))}{d\gamma} + \sum_{i=1}^r N_i(\gamma) \frac{d\mu_S^i(\vec{Y}(\gamma))}{d\gamma},$$

$$0 = \frac{dT_S}{d\gamma}(\vec{Y}(\gamma)) \tilde{S}(\vec{Y}(\gamma)) - \frac{dP_S}{d\gamma}(\vec{Y}(\gamma)) V(\gamma) + \sum_{j=1}^r \frac{d\mu_S^j}{d\gamma}(\vec{Y}(\gamma)) N_j(\gamma),$$

These are essentially the same expression!

Math Thermo

Class #04

01/29/2026

Suppose that  $\tilde{S}$  is the fundamental entropy relation for an isolated system containing a unary ( $r = 1$ ) material.

$$\tilde{S} = \tilde{S}(U, V, N).$$

Suppose that  $N > 0$  is fixed. Define

$$u := \frac{U}{N}, \quad \text{the molar energy,}$$

$$v := \frac{V}{N}, \quad \text{the molar volume.}$$

Then, since, for any  $\lambda > 0$ ,

$$\lambda \tilde{S}(U, V, N) = \tilde{S}(\lambda U, \lambda V, \lambda N),$$

it follows that

$$\frac{1}{N} \tilde{S}(U, V, N) = \tilde{S}\left(\frac{U}{N}, \frac{V}{N}, \frac{N}{N}\right) = \tilde{S}(u, v, 1).$$

Now, define the molar entropy relation

$$\tilde{s} = \tilde{s}(u, v) := \tilde{S}(u, v, 1).$$

It then follows that

$$\tilde{S}(U, V, N) = N \tilde{s}(u, v).$$

Likewise, if we define

$$s = \frac{S}{N} \quad v = \frac{V}{N}$$

and

$$\tilde{u} = \tilde{u}(s, v) := \tilde{U}(s, v, 1),$$

then it follows that

$$\tilde{U}(S, V, N) = N\tilde{u}(s, v).$$

**Example 1.3.2.** (4.1) Suppose that

$$\tilde{S}(U, V, N) = \left( \frac{NVUR^2}{v_0\theta} \right)^{1/3},$$

where  $R, v_0, \theta > 0$  are constants. Then,

$$\tilde{s}(u, v) = \tilde{S}(u, v, 1) = \left( \frac{vuR^2}{v_0\theta} \right)^{1/3}.$$

$$N\tilde{s}(u, v) = \left( \frac{N^3vuR^2}{v_0\theta} \right)^{1/3} = \left( \frac{NVUR^2}{v_0\theta} \right)^{1/3} = \tilde{S}(U, V, N).$$

$\tilde{U}$  and  $\tilde{S}$  are homogeneous of degree one (also called extensive variables).

$T, P, \mu$  on the other hand are homogeneous of degree zero (also called intensive variables).

Recall that, for all  $\lambda > 0$ ,

$$T_U(S, V, N) = T_U(\lambda S, \lambda V, \lambda N).$$

Thus,

$$T_U(S, V, N) = T_U(s, v, 1).$$

We could, of course, give a new symbol for  $T_U(s, v, 1)$ , for example

$$t_U(s, v) := T_U(s, v, 1) \dots$$

## 1.4 Molar Euler and Gibbs–Duhem Equation

For a unary material ( $r = 1$ ), recall

$$\tilde{U}(S, V, N) = T_U(S, V, N)S - P_U(S, V, N)V + \mu_U(S, V, N)N$$

Suppose  $N > 0$  is fixed. Then,

$$\frac{1}{N}\tilde{U}(S, V, N) = T_U(S, V, N)\frac{S}{N} - P_U(S, V, N)\frac{V}{N} + \mu_U(S, V, N)$$

or, equivalently,

$$\tilde{u}(s, v) = T_U(s, v)s - P_U(s, v)v + \mu_U(s, v). \quad (4.1)$$

This is the molar version of Euler's equation. How do we get the Gibbs–Duhem equation?

Let  $\vec{z}(\gamma) = (s(\gamma), v(\gamma))$  be a path in molar state space. Then

$$\frac{d}{d\gamma} \tilde{u}(\vec{z}(\gamma)) = \frac{\partial \tilde{u}}{\partial s}(\vec{z}(\gamma)) s'(\gamma) + \frac{\partial \tilde{u}}{\partial v}(\vec{z}(\gamma)) v'(\gamma).$$

But  
exercise

$$\frac{\partial \tilde{u}}{\partial s}(\vec{z}(\gamma)) = T_U(s(\gamma), v(\gamma))$$

and

$$\frac{\partial \tilde{u}}{\partial v}(\vec{z}(\gamma)) = -P_U(s(\gamma), v(\gamma)).$$

Thus, the combined First and Second laws are

$$\frac{d}{d\gamma} \tilde{u}(\vec{z}(\gamma)) = T_U(\vec{z}(\gamma))s'(\gamma) - P_U(\vec{z}(\gamma))v'(\gamma). \quad (4.2)$$

On the other hand, differentiate the molar Euler relation (4.1), we have

$$\frac{d}{d\gamma} \tilde{u}(\vec{z}(\gamma)) = \frac{d}{d\gamma} T_U(\vec{z}(\gamma))s(\gamma) + T_U(\vec{z}(\gamma))s'(\gamma) \quad (1.4.1)$$

$$- \frac{d}{d\gamma} P_U(\vec{z}(\gamma))v(\gamma) - P_U(\vec{z}(\gamma))v'(\gamma) \quad (1.4.2)$$

$$+ \frac{d}{d\gamma} \mu_U(\vec{z}(\gamma)). \quad (4.3)$$

Therefore, the molar Gibbs–Duhem equation is

$$0 = \frac{d}{d\gamma} T_U(\vec{z}(\gamma))s(\gamma) - \frac{d}{d\gamma} P_U(\vec{z}(\gamma))v(\gamma) + \frac{d}{d\gamma} \mu_U(\vec{z}(\gamma)). \quad (4.4)$$

The molar entropy form of the Euler and Gibbs–Duhem equations are (as one would expect)

$$\tilde{s}(u, v) = \frac{1}{T_S(u, v)} u + \frac{P_S(u, v)}{T_S(u, v)} v - \frac{\mu_S(u, v)}{T_S(u, v)}. \quad (4.6)$$

and

$$0 = \frac{d}{d\gamma} \left( \frac{1}{T_S(\vec{z}(\gamma))} \right) u(\gamma) + \frac{d}{d\gamma} \left( \frac{P_S(\vec{z}(\gamma))}{T_S(\vec{z}(\gamma))} \right) v(\gamma) - \frac{d}{d\gamma} \left( \frac{\mu_S(\vec{z}(\gamma))}{T_S(\vec{z}(\gamma))} \right). \quad (4.7)$$

The molar representation of the First and Second laws is

$$\frac{d}{d\gamma} \tilde{s}(\vec{z}(\gamma)) = \frac{1}{T_S(\vec{z}(\gamma))} u'(\gamma) + \frac{P_S(\vec{z}(\gamma))}{T_S(\vec{z}(\gamma))} v'(\gamma). \quad (4.8)$$

where  $\vec{z}(\gamma) = (u(\gamma), v(\gamma))$  is a process path in molar state space.

## 1.5 Examples

Let's look at a couple of examples.

**Example 1.5.1.** (4.2) Suppose that

$$P = \frac{2U}{V}$$

$$T = \left( \frac{AU^{3/2}}{VN^{1/2}} \right)^{1/2}$$

(homog. deg. zero)

We should be able to recover the fundamental relation using these two equations of state. Observe that

$$\frac{1}{T_S} = A^{-1/2} u^{-3/4} v^{1/2}$$

$$\frac{P_S}{T_S} = 2A^{-1/2} u^{1/4} v^{-1/2}$$

Using the molar 1st and 2nd laws (4.8)

$$\begin{aligned} \frac{d}{d\gamma} \tilde{s}(\vec{z}(\gamma)) &= \frac{1}{T_S(\vec{z}(\gamma))} u'(\gamma) + \frac{P_S(\vec{z}(\gamma))}{T_S(\vec{z}(\gamma))} v'(\gamma) \\ &= A^{-1/2} \left( u(\gamma)^{-3/4} v(\gamma)^{1/2} u'(\gamma) + 2u(\gamma)^{1/4} v(\gamma)^{-1/2} v'(\gamma) \right) \\ &= 4A^{-1/2} \frac{d}{d\gamma} \left( (u(\gamma))^{1/4} (v(\gamma))^{1/2} \right). \end{aligned}$$

Therefore,

$$\tilde{s}(\gamma) = 4A^{-1/2}(u(\gamma))^{1/4}(v(\gamma))^{1/2} + s_0.$$

Equivalently,

$$\tilde{S}(\gamma) = 4A^{-1/2}U^{1/4}V^{1/2}N^{1/4} + Ns_0.$$

here  $s_0$  is a positive constant. ///

Let's try an alternative method.

**Example 1.5.2.** (4.3) Same problem as above. This time we will use the Gibbs–Duhem equation (4.7) as the starting point:

$$\begin{aligned} \frac{d}{d\gamma} \left( \frac{\mu_S(\vec{z}(\gamma))}{T_S(\vec{z}(\gamma))} \right) &= \frac{d}{d\gamma} \left( \frac{1}{T_S(\vec{z}(\gamma))} \right) u(\gamma) + \frac{d}{d\gamma} \left( \frac{P_S(\vec{z}(\gamma))}{T_S(\vec{z}(\gamma))} \right) v(\gamma) \\ &= A^{-1/2} \frac{d}{d\gamma} \left( (u(\gamma))^{-3/4} (v(\gamma))^{1/2} \right) u(\gamma) \\ &\quad + A^{-1/2} \frac{d}{d\gamma} \left( 2(u(\gamma))^{1/4} (v(\gamma))^{-1/2} \right) v(\gamma) \\ &= A^{-1/2} \left( -\frac{3}{4} (u(\gamma))^{-3/4} (v(\gamma))^{1/2} u'(\gamma) \right. \\ &\quad \left. + (u(\gamma))^{1/4} \frac{1}{2} (v(\gamma))^{-1/2} v'(\gamma) \right) \\ &\quad + A^{-1/2} \left( \frac{1}{2} (u(\gamma))^{-3/4} (v(\gamma))^{1/2} u'(\gamma) \right. \\ &\quad \left. - 2(u(\gamma))^{1/4} \frac{1}{2} (v(\gamma))^{-1/2} v'(\gamma) \right) \\ &= A^{-1/2} \left( -\frac{1}{4} (u(\gamma))^{-3/4} (v(\gamma))^{1/2} u'(\gamma) \right. \\ &\quad \left. - \frac{1}{2} (u(\gamma))^{1/4} (v(\gamma))^{-1/2} v'(\gamma) \right) \\ &= -A^{-1/2} \frac{d}{d\gamma} \left( (u(\gamma))^{1/4} (v(\gamma))^{1/2} \right). \end{aligned}$$

Thus,

$$\frac{\mu_S(\vec{z}(\gamma))}{T_S(\vec{z}(\gamma))} = -A^{-1/2}(u(\gamma))^{1/4}(v(\gamma))^{1/2} - s_0.$$



or

$$\frac{\mu_S(u, v)}{T_S(u, v)} = -A^{-1/2}u^{1/4}v^{1/2} - s_0.$$

Using Euler's equation (4.6), we have

$$\begin{aligned}\tilde{s}(u, v) &= \frac{1}{T_S(u, v)}u + \frac{P_S(u, v)}{T_S(u, v)}v - \frac{\mu_S(u, v)}{T_S(u, v)} \\ &= A^{-1/2}u^{1/4}v^{1/2} + 2A^{-1/2}u^{1/4}v^{1/2} + A^{-1/2}u^{1/4}v^{1/2} + s_0 \\ &= 4A^{-1/2}u^{1/4}v^{1/2} + s_0,\end{aligned}$$

which is the same as before.

Using 2 equations of state, we can recover the 3rd and then utilizing Euler's equation we get the fundamental relation. ///

**Example 1.5.3.** (4.4) Ideal Gas law

$$PV = NRT$$

$$U = \frac{3}{2}NRT$$

With these two equations of state we can find the fundamental relations.

Observe that

$$\frac{1}{T_S} = \frac{3R}{2u} \quad \frac{P_S}{T_S} = \frac{R}{v}.$$

This suggests that we again use the entropy equation (in molar form). The Gibbs–Duhem equation is

$$\begin{aligned}\frac{d}{d\gamma} \left( \frac{\mu_S(\vec{z}(\gamma))}{T_S(\vec{z}(\gamma))} \right) &= \frac{d}{d\gamma} \left( \frac{1}{T_S(\vec{z}(\gamma))} \right) u(\gamma) + \frac{d}{d\gamma} \left( \frac{P_S(\vec{z}(\gamma))}{T_S(\vec{z}(\gamma))} \right) v(\gamma) \\ &= \frac{3R}{2} \frac{d}{d\gamma} \left( \frac{1}{u(\gamma)} \right) u(\gamma) + R \frac{d}{d\gamma} \left( \frac{1}{v(\gamma)} \right) v(\gamma) \\ &= -\frac{3R}{2} \frac{u'(\gamma)}{u(\gamma)} - R \frac{v'(\gamma)}{v(\gamma)}.\end{aligned}$$

Integrating, we have

$$\frac{\mu_S(u(\gamma), v(\gamma))}{T_S(u(\gamma), v(\gamma))} - \frac{\mu_0}{T_0} = -\frac{3R}{2} \ln \left( \frac{u(\gamma)}{u_0} \right) - R \ln \left( \frac{v(\gamma)}{v_0} \right),$$

where

$$\frac{\mu_0}{T_0} := \frac{\mu_S(u_0, v_0)}{T_S(u_0, v_0)}.$$

Using the molar Euler equation, we have

$$\begin{aligned}\tilde{s}(u, v) &= \frac{1}{T_S(u, v)}u + \frac{P_S(u, v)}{T_S(u, v)}v - \frac{\mu_S(u, v)}{T_S(u, v)} \\ &= \frac{3R}{2} + R + \frac{3R}{2} \ln \left( \frac{u}{u_0} \right) + R \ln \left( \frac{v}{v_0} \right) - \frac{\mu_0}{T_0} \\ &= s_0 + R \ln \left( \left( \frac{u}{u_0} \right)^{3/2} \left( \frac{v}{v_0} \right) \right).\end{aligned}$$

Thus,

$$\tilde{S}(U, V, N) = Ns_0 + NR \ln \left( \left( \frac{U}{U_0} \right)^{3/2} \left( \frac{V}{V_0} \right) \left( \frac{N}{N_0} \right)^{-5/2} \right),$$

where

$$U = uN, \quad V = vN,$$

$$U_0 = u_0N_0, \quad V_0 = v_0N_0,$$

and

$$s_0 = \frac{5}{2}R - \frac{\mu_0}{T_0}.$$